refactor

theories/examples/approximate_bounded_rejection_sampler.v
@@ -66,48 +66,6 @@ Section basic.
 
   (** PROBLEM 1: show the bounded sampler terminates inbounds with some error *)
 
-  (** nnreal exponents *)
-  Fixpoint nnreal_nat_exp (r : nonnegreal) (n : nat) : nonnegreal :=
-    match n with
-    | O    => nnreal_one
-    | S n' => nnreal_mult r (nnreal_nat_exp r n')
-    end.
-
-  Lemma nnreal_nat_exp_bound (r : nonnegreal) (Hr : r < 1) (n : nat) : nnreal_nat_exp r (S n) < 1.
-  Proof.
-    induction n as [|n' IH].
-    - simpl; by rewrite Rmult_1_r.
-    - remember (S n') as nₛ.
-      simpl.
-      apply (Rcomplements.Rle_mult_Rlt r).
-      + apply Rlt_0_1.
-      + auto.
-      + replace (1 * nonneg r) with (nonneg r * 1); last first.
-        { rewrite -> Rmult_1_r; rewrite -> Rmult_1_l; done. }
-        apply Rmult_le_compat_l; try (by apply Rlt_le).
-        apply cond_nonneg.
-  Qed.
-
-  Lemma nnreal_nat_exp_limit : forall (r 𝜀 : nonnegreal), (* (0 < 𝜀) -> (𝜀 < 1) -> (0 < r) -> *) (r < 1) -> exists n, forall n0, (n0 > n)%nat -> (nnreal_nat_exp r n0) < 𝜀.
-  Proof.
-    (*
-    intros r 𝜀 H𝜀L HεU HrL HrU.
-    exists (Z.to_nat $ up $ Rlog r 𝜀).
-    intros n0 Hn0.
-    induction n0 as [| n0' Hn0'].
-    - simpl. lia.
-    - simpl.
-      rewrite -> Rcomplements.Rlt_div_r; last first.
-      { induction n0' as [|m Hm].
-        + simpl; apply Rlt_gt; apply Rlt_0_1.
-        + simpl; apply Rlt_gt; apply Rmult_lt_0_compat; auto; apply Rgt_lt. apply Hm; [admit | admit].
-
-     this proof is a mess and is going nowhere*)
-
-    (* use an actual limit thm. *)
-  Admitted.
-
-
   (** defining error values for each step *)
 
   Definition err_factor n m := (nnreal_div (nnreal_nat (m - n)%nat) (nnreal_nat m%nat)).
@@ -143,22 +101,25 @@ Section basic.
 
 
   (* error for the bounded sampler with a given number of tries remaining *)
-  Definition bdd_cf_error n m depth := nnreal_nat_exp (err_factor n m) depth.
+  Program Definition bdd_cf_error n m depth (Hnm : (n < m)%nat) := mknonnegreal ((err_factor n m) ^ depth) _.
+  Next Obligation.
+    intros.
+    apply pow_le; rewrite /err_factor /=.
+    apply Rle_mult_inv_pos.
+    - apply pos_INR.
+    - apply lt_0_INR; lia.
+  Qed.
 
   (* this lemma is for proofs which iterate to the very end
      ie, doing 0 samples requires error tolerance of 1 *)
-  Lemma bdd_cd_error_final n m : bdd_cf_error n m 0 = nnreal_one.
-  Proof. by rewrite /bdd_cf_error /nnreal_nat_exp. Qed.
+  Lemma bdd_cd_error_final n m (Hnm : (n < m)%nat) : bdd_cf_error n m 0 Hnm = nnreal_one.
+  Proof. by apply nnreal_ext; simpl. Qed.
 
   (* this lemma is for proofs which iterate up until the last sample
      ie, a rejection sampler to exclude the final recursive step *)
   (* proof irrelevant *)
-  Lemma bdd_cd_error_penultimate n m : bdd_cf_error n m 1 = err_factor n m.
-  Proof.
-    rewrite /bdd_cf_error /nnreal_nat_exp.
-    apply nnreal_ext.
-    simpl; by apply Rmult_1_r.
-  Qed.
+  Lemma bdd_cd_error_penultimate n m (Hnm : (n < m)%nat) : bdd_cf_error n m 1 Hnm = err_factor n m.
+  Proof. apply nnreal_ext; simpl; apply Rmult_1_r. Qed.
 
 
   (* distribution of error mass 𝜀₁ for a given sample:
@@ -172,24 +133,31 @@ Section basic.
 
   (* lemma for simplifying accumulated error in the recursive case *)
   Lemma simplify_accum_err (n m d': nat) (Hnm : (n < m)%nat) (s : fin m)  :
-    (s <? n)%nat = false -> bdd_cf_sampling_error n m (bdd_cf_error n m (S d')) s = (bdd_cf_error n m d' ).
+    (s <? n)%nat = false -> bdd_cf_sampling_error n m (bdd_cf_error n m (S d') Hnm) s = (bdd_cf_error n m d' Hnm).
   Proof.
     intros Hcase.
-    rewrite /bdd_cf_sampling_error Hcase /bdd_cf_error {1}/nnreal_nat_exp -/nnreal_nat_exp.
-    remember (err_factor n m) as X.
-    remember (nnreal_nat_exp X d') as Y.
-    apply nnreal_ext; simpl.
-    replace (X * Y) with (Y * X) by apply Rmult_comm.
-    apply Rinv_r_simpl_l.
-    rewrite HeqX.
-    rewrite /not; intros; apply (err_factor_nz n m Hnm).
-    simpl. apply nnreal_ext.
-    by replace (nonneg nnreal_zero) with 0 by auto.
+    apply nnreal_ext.
+    rewrite /bdd_cf_sampling_error Hcase /bdd_cf_error /=.
+    apply Rinv_r_simpl_m.
+    by apply err_factor_nz_R.
+  Qed.
+
+
+  Lemma factor_lt_1 n m (Hnm : (n < m)%nat) (Hn : (0 < n)%nat): ((m - n)%nat  * / m) < 1.
+  Proof.
+    apply (Rmult_lt_reg_l m); first (apply lt_0_INR; lia).
+    rewrite Rmult_1_r.
+    replace (m * (INR ((m-n)%nat) * / m)) with (INR (m-n)%nat); last first.
+    - rewrite Rmult_comm.
+      rewrite Rmult_assoc.
+      replace (/m * m) with 1; last by (symmetry; apply Rinv_l; apply not_0_INR; lia).
+      symmetry; apply Rmult_1_r.
+    - apply lt_INR. lia.
   Qed.
 
 
   (* error distribution is well-formed for each possible sample *)
-  Lemma sample_err_wf n m d (s : fin m) (Hn : (0 < n)%nat) (Hnm : (n < m)%nat) : bdd_cf_sampling_error n m (bdd_cf_error n m (S d)) s <= 1.
+  Lemma sample_err_wf n m d (s : fin m) (Hn : (0 < n)%nat) (Hnm : (n < m)%nat) : bdd_cf_sampling_error n m (bdd_cf_error n m (S d) Hnm) s <= 1.
   Proof.
     (* it is either 1, or epsilon times something at most 1 *)
     rewrite /bdd_cf_sampling_error.
@@ -199,21 +167,13 @@ Section basic.
     - rewrite -> Rinv_r_simpl_m.
       + destruct d as [|d'].
         * simpl; apply Rge_refl.
-        * apply Rlt_le. apply nnreal_nat_exp_bound. apply err_factor_lt1; done.
+        * apply Rlt_le.
+          apply pow_lt_1_compat; try lia; split.
+          -- apply Rle_mult_inv_pos; [ apply pos_INR | apply lt_0_INR; lia ].
+          -- apply factor_lt_1; auto.
       + apply err_factor_nz_R; auto.
   Qed.
 
-      (* lemma: the geometric factor is less than 1
-      assert (Hfc : ((m - n)%nat  * / m) < 1).
-      { apply (Rmult_lt_reg_l m); first (apply lt_0_INR; lia).
-        rewrite Rmult_1_r.
-        replace (m * (INR ((m-n)%nat) * / m)) with (INR (m-n)%nat); last first.
-        { rewrite Rmult_comm.
-          rewrite Rmult_assoc.
-          replace (/m * m) with 1; last by (symmetry; apply Rinv_l; apply not_0_INR; lia).
-          symmetry; apply Rmult_1_r. }
-        apply lt_INR; lia. }
-      *)
 
   (* mean of error distribution is preserved *)
   Lemma sample_err_mean n' m' 𝜀₁ :
@@ -233,21 +193,21 @@ Section basic.
   (** warmup: a finite example *)
   Definition bdd_approx_safe_finite_example (n' m' depth : nat) (Hnm : (S n' < S m')%nat) E :
     (depth = 3%nat) ->
-    {{{ € (bdd_cf_error (S n') (S m') depth) }}} bdd_rejection_sampler n' m' #(S depth) @ E {{{ v, RET v ; ⌜exists v' : nat, v = SOMEV #v' /\ (v' < S n')%nat⌝ }}}.
+    {{{ € (bdd_cf_error (S n') (S m') depth Hnm) }}} bdd_rejection_sampler n' m' #(S depth) @ E {{{ v, RET v ; ⌜exists v' : nat, v = SOMEV #v' /\ (v' < S n')%nat⌝ }}}.
   Proof.
     (* make these off by one errors easier to unpack *)
-    remember (S n') as n.
+    (* remember (S n') as n.
     remember (S m') as m.
     assert (Hn : (0 < n)%nat) by lia.
-    assert (Hm : (0 < m)%nat) by lia.
+    assert (Hm : (0 < m)%nat) by lia. *)
 
     iIntros (-> Φ) "Hcr HΦ"; rewrite /bdd_rejection_sampler.
-    wp_pures. rewrite Heqm Heqn.
+    wp_pures. (* rewrite Heqm. Heqn. *)
 
     (* S depth=3 sample *)
     wp_apply (wp_couple_rand_adv_comp _ _ _ Φ _ (bdd_cf_sampling_error (S n') _ _) with "Hcr").
     { intros s. apply sample_err_wf; try lia. }
-    { pose P := (sample_err_mean n' m' (bdd_cf_error (S n') (S m') 3)); apply P. }
+    { pose P := (sample_err_mean n' m' (bdd_cf_error (S n') (S m') 3 Hnm)); apply P. }
     iIntros (sample) "Hcr".
     wp_pures.
     case_bool_decide; wp_pures.
@@ -257,7 +217,7 @@ Section basic.
     (* S depth=2 sample *)
     wp_apply (wp_couple_rand_adv_comp _ _ _ Φ _ (bdd_cf_sampling_error (S n') _ _) with "Hcr").
     { intros s. apply sample_err_wf; try lia. }
-    { pose P := (sample_err_mean n' m' (bdd_cf_error (S n') (S m') 2)); apply P. }
+    { pose P := (sample_err_mean n' m' (bdd_cf_error (S n') (S m') 2 Hnm)); apply P. }
     iIntros (sample') "Hcr".
     wp_pures.
     case_bool_decide; wp_pures.
@@ -266,7 +226,8 @@ Section basic.
 
     (* S depth=1 sample *)
     rewrite bdd_cd_error_penultimate.
-    rewrite -Heqm -Heqn.
+    remember (S n') as n.
+    remember (S m') as m.
     wp_apply (wp_rand_err_list_nat _ m' (seq n (m - n))).
     iSplitL "Hcr".
     - (* yeesh *)
@@ -291,13 +252,8 @@ Section basic.
 
   (** general case for the bounded sampler *)
   Definition bdd_approx_safe (n' m' depth : nat) (Hnm : (S n' < S m')%nat) E :
-    {{{ € (bdd_cf_error (S n') (S m') (S depth)) }}} bdd_rejection_sampler n' m' #(S depth)@ E {{{ v, RET v ; ⌜exists v' : nat, v = SOMEV #v' /\ (v' < S n')%nat⌝ }}}.
+    {{{ € (bdd_cf_error (S n') (S m') (S depth) Hnm) }}} bdd_rejection_sampler n' m' #(S depth)@ E {{{ v, RET v ; ⌜exists v' : nat, v = SOMEV #v' /\ (v' < S n')%nat⌝ }}}.
   Proof.
-    remember (S n') as n.
-    remember (S m') as m.
-    assert (Hn : (0 < n)%nat) by lia.
-    assert (Hm : (0 < m)%nat) by lia.
-
     iIntros (Φ) "Hcr HΦ"; rewrite /bdd_rejection_sampler.
     do 4 wp_pure.
 
@@ -305,6 +261,8 @@ Section basic.
     iInduction depth as [|depth' Hdepth'] "IH".
     - wp_pures.
       rewrite bdd_cd_error_penultimate.
+      remember (S n') as n.
+      remember (S m') as m.
       wp_apply (wp_rand_err_list_nat _ m' (seq n (m - n))).
       iSplitL "Hcr".
       + rewrite /err_factor.
@@ -328,7 +286,7 @@ Section basic.
       wp_pures.
       wp_apply (wp_couple_rand_adv_comp _ _ _ Φ _ (bdd_cf_sampling_error (S n') _ _) with "Hcr").
       { intros s. apply sample_err_wf; try lia. }
-      { pose P := (sample_err_mean n' m' (bdd_cf_error (S n') (S m') _)); rewrite Heqn Heqm; by eapply P. }
+      { pose P := (sample_err_mean n' m' (bdd_cf_error (S n') (S m') _ Hnm)); by eapply P. }
       iIntros (sample') "Hcr".
       wp_pures.
       case_bool_decide.
@@ -337,7 +295,6 @@ Section basic.
         rewrite (simplify_accum_err (S n') (S m') _); last (apply Nat.ltb_nlt; by lia); try lia.
         wp_bind (#_ - #_)%E. wp_pure.
         replace (S (S depth') - 1)%Z with (Z.of_nat (S depth')) by lia.
-        rewrite Heqn Heqm.
         wp_apply ("IH" with "Hcr HΦ").
   Qed.
 
@@ -345,19 +302,16 @@ Section basic.
 
   (** PROBLEM 3: show that the unbounded approximate sampler is safe if we have enough error to eliminate past a depth *)
   Definition ubdd_approx_safe (n' m' depth : nat) (Hnm : (S n' < S m')%nat) E :
-    {{{ € (bdd_cf_error (S n') (S m') (S depth)) }}} ubdd_rejection_sampler n' m' #() @ E {{{ v, RET v ; ⌜exists v' : nat, v = SOMEV #v' /\ (v' < S n')%nat⌝  }}}.
+    {{{ € (bdd_cf_error (S n') (S m') (S depth) Hnm) }}} ubdd_rejection_sampler n' m' #() @ E {{{ v, RET v ; ⌜exists v' : nat, v = SOMEV #v' /\ (v' < S n')%nat⌝  }}}.
   Proof.
-    remember (S n') as n.
-    remember (S m') as m.
-    assert (Hn : (0 < n)%nat) by lia.
-    assert (Hm : (0 < m)%nat) by lia.
-
     iIntros (Φ) "Hcr HΦ"; rewrite /ubdd_rejection_sampler.
     do 4 wp_pure.
 
     iInduction depth as [|depth' Hdepth'] "IH".
     - wp_pures.
       rewrite bdd_cd_error_penultimate.
+      remember (S n') as n.
+      remember (S m') as m.
       wp_apply (wp_rand_err_list_nat _ m' (seq n (m - n))).
       iSplitL "Hcr".
       + rewrite /err_factor.
@@ -379,14 +333,13 @@ Section basic.
     - wp_pures.
       wp_apply (wp_couple_rand_adv_comp _ _ _ Φ _ (bdd_cf_sampling_error (S n') _ _) with "Hcr").
       { intros s. apply sample_err_wf; try lia. }
-      { pose P := (sample_err_mean n' m' (bdd_cf_error (S n') (S m') _)); rewrite Heqn Heqm; by eapply P. }
+      { pose P := (sample_err_mean n' m' (bdd_cf_error (S n') (S m') _ Hnm));  by eapply P. }
       iIntros (sample') "Hcr".
       wp_pures.
       case_bool_decide.
       + wp_pures. iApply "HΦ"; iModIntro; iPureIntro; exists (fin_to_nat sample'); split; [auto|lia].
       + wp_pure.
         rewrite (simplify_accum_err (S n') (S m') _); last (apply Nat.ltb_nlt; by lia); try lia.
-        rewrite Heqn Heqm.
         wp_apply ("IH" with "Hcr HΦ").
   Qed.
 
@@ -396,6 +349,9 @@ Section basic.
     ⊢ {{{ €𝜀 ∗ ⌜𝜀 > 0 ⌝  }}} ubdd_rejection_sampler n' m' #()@ E {{{ v, RET v ; ⌜exists v' : nat, v = SOMEV #v' /\ (v' < S n')%nat⌝ }}}.
   Proof.
     iIntros (𝜀 Φ) "!> (Hcr&%Hcrpos) HΦ".
+
+    Admitted.
+  (*
     destruct (nnreal_nat_exp_limit (err_factor (S n') (S m')) 𝜀) as [d].
     - apply err_factor_lt1; lia.
     - iApply (ubdd_approx_safe with "[Hcr] [HΦ]"); auto.
@@ -403,6 +359,6 @@ Section basic.
       rewrite /bdd_cf_error.
       apply Rlt_le.
       specialize H with (S d); apply H; lia.
-  Qed.
+  Qed. *)
 
 End basic.
